\let\negmedspace\undefined
\let\negthickspace\undefined
\documentclass{beamer}
\usetheme{CambridgeUS}
\usepackage{csquotes}
\usepackage{comment}
\usepackage{enumerate}
\usepackage{amsmath,amssymb,amsthm}
\usepackage{graphicx}
\let\vec\mathbf
\newcommand{\myvec}[1]{\ensuremath{\begin{pmatrix}#1\end{pmatrix}}}
\providecommand{\brak}[1]{\ensuremath{\left(#1\right)}}
\providecommand{\pr}[1]{\ensuremath{\Pr\left(#1\right)}}


     \title{Assignment 8}
     \author{AKKASANI YAGNESH REDDY \\
     CS21BTECH11003 }
     \date{\today}
\logo{\large \LaTeX{}}
     
     \begin{document}
     \begin{frame}
     \maketitle    
     \end{frame}
     
     \logo{}
     
     \begin{frame}{Outline}
    \tableofcontents
     \end{frame}
     
     
     \section{Question}
     \begin{frame}
         \textbf{Question:}Show that if $F(x, y, z)$ is a joint distribution. then for any $x_{1}\leq x_{2},y_{1}\leq y_{2},z_{1}\leq z_{2}$:
     \begin{align}
         F(x_{2},y_{2},z_{2})+F(x_{1},y_{1},z_{1})+F(x_{1},y_{2},z_{1})\nonumber\\+F(x_{2},y_{1},z_{1})-F(x_{1},y_{2},z_{2})-F(x_{2},y_{1},z_{2})\nonumber\\-F(x_{2},y_{2},z_{1})-F(x_{1},y_{1},z_{1})\geq 0
         \end{align}
     \end{frame}
     
     \section{Solution:}\begin{frame}
       \textbf{Solution:}We know that,
    Using this instead of $F$,
     \begin{align}
        F(x)=\pr{X\leq x}
    \end{align}
  \begin{align}
0 \leq \pr{x_{1}\leq x\leq x_{2},y_{1}\leq y\leq y_{2},z_{1}\leq z\leq z_{2}}\\
0\leq\pr{x\leq x_{2},y_{1}\leq y\leq y_{2},z_{1}\leq z\leq z_{2}}\nonumber\\-\pr{x\leq x_{1},y_{1}\leq y\leq y_{2},z_{1}\leq z\leq z_{2}}
        \end{align}
          \end{frame}
          \begin{frame}
          \begin{align}
               =\pr{x\leq x_{2},y\leq y_{2},z_{1}\leq z\leq z_{2}}
        -\pr{x\leq x_{2},y\leq y_{1},z_{1}\leq z\leq z_{2}}\nonumber\\
        -\pr{x\leq x_{1},y\leq y_{2},z_{1}\leq z\leq z_{2}}
        +\pr{x\leq x_{1},y\leq y_{1},z_{1}\leq z\leq z_{2}}
           \end{align}
          \end{frame}
          
          \begin{frame}
          \begin{align}
          =\pr{x\leq x_{2},y\leq y_{2},z\leq z_{2}}
        -\pr{x\leq x_{2},y\leq y_{2},z\leq z_{1}}\nonumber\\
        -\pr{x\leq x_{2},y\leq y_{1},z\leq z_{2}}
        +\pr{x\leq x_{2},y\leq y_{1},z\leq z_{1}}\nonumber\\
        -\pr{x\leq x_{1},y\leq y_{2},z\leq z_{2}}
        +\pr{x\leq x_{1},y\leq y_{2},z\leq z_{1}}\nonumber\\
        +\pr{x\leq x_{1},y\leq y_{1},z\leq z_{2}}
        -\pr{x\leq x_{1},y\leq y_{1},z\leq z_{1}}
        \end{align}
              \end{frame}
              \begin{frame}
              Hence proved because the above is $\geq0$ and is same as given in question that is,
         \begin{align}
         F(x_{2},y_{2},z_{2})+F(x_{1},y_{1},z_{1})+F(x_{1},y_{2},z_{1})\nonumber\\+F(x_{2},y_{1},z_{1})-F(x_{1},y_{2},z_{2})-F(x_{2},y_{1},z_{2})\nonumber\\-F(x_{2},y_{2},z_{1})-F(x_{1},y_{1},z_{1})\geq 0
         \end{align}
                  
              \end{frame}
              
     
 \end{document}